% !TeX root = ./TMA04.tex

Using the result obtained in part~(b) it will be shown that for a stationary path of $S$ that
\begin{equation}
	\pderiv{L}{t} = -\dot{H}
\end{equation}
as follows.
\begin{align*}
	\deriv{H}{t} &= \deriv{}{t}\lr{p\dot{x} - L},\\
	&= \deriv{}{t}\lr{p\dot{x}} -\deriv{L}{t},\\
	&= p\ddot{x} + p\dot{x} -\deriv{L}{t},\\
	\text{and }&\text{substituting into the above expression for } \deriv{L}{t} \text{ from part~(b) gives,}\\
	&= p\ddot{x} + p\dot{x} - \lr{\pderiv{L}{t} + \pderiv{L}{x}\dot{x} + p\ddot{x}},\\
	&= \cancel{p\ddot{x}} + \cancel{p\dot{x}} - \lr{\pderiv{L}{t} + \cancel{\dot{p}\dot{x}} + \cancel{p\ddot{x}}},\\
	\therefore \deriv{H}{t} =\dot{H} &= -\pderiv{L}{t},\qtq{as required.}
\end{align*}
