% !TeX root = ./TMA04.tex
The Rund-Trautman Identity:
\begin{align}
\label{5.5}
	\pderiv{L}{x}\xi +  \boxed{p\dot{\xi}} + \pderiv{L}{t}\tau - \boxed{H\dot{\tau}}=0,\\
\label{5.6}
	-\pderiv{L}{x}\xi - \pderiv{L}{t}\tau = \boxed{p\dot{\xi}  - H\dot{\tau}}.
\end{align}
The RHS of \eqref{eq:5.4} can be expanded using the product rule,
\begin{align}
\label{5.7}
	\deriv{}{t}\lrs{p\xi-H\tau} &= \boxed{p\dot{\xi}} +\dot{p}\xi - \boxed{H\dot{\tau}} - \dot{H}\tau,\\
\label{5.8}
	\deriv{}{t}\lrs{p\xi-H\tau} &= \boxed{p\dot{\xi} - H\dot{\tau}} - \dot{H}\tau +\dot{p}\xi.
\end{align}
Substituting for $\boxed{p\dot{\xi} - h\dot{\tau}}$ from \eqref{5.6} into \eqref{5.8} gives,
\begin{align}
\label{5.9}
	\deriv{}{t}\lrs{p\xi-H\tau}&= -\pderiv{L}{x}\xi - \pderiv{L}{t}\tau  - \dot{H}\tau +\dot{p}\xi,
\end{align}
and collecting like terms in $\xi$,
\begin{align}
\label{5.10}
	\deriv{}{t}\lrs{p\xi-H\tau}&=  \xi\lr{\dot{p} -\pderiv{L}{x}} - \pderiv{L}{t}\tau  - \dot{H}\tau.
\end{align}
From the question (preamble to part~(c)), the \textit{Hamiltonian} is defined as
\begin{align}
\label{5.11}
	H &= p\dot{x} - L,\qtq{and its derivative is given by}\\
\label{5.12}
	\deriv{H	}{t} &= \dot{H} = \deriv{}{t}\lr{p\dot{x}}-\deriv{L}{t},\\
\label{5.13}
	\deriv{H	}{t} &= p\ddot{x} +\dot{p}\dot{x} -\deriv{L}{t}.
\end{align}
As shown in part~(b),
\begin{align}
\label{5.14}
\deriv{L}{t} &= \pderiv{L}{t}+\pderiv{L}{x}\dot{x} + p\ddot{x}.
\end{align}
Substituting for $\dd L/\dd t$ in \eqref{5.13} from \eqref{5.14} gives,
\begin{align}
\label{5.15}
	\dot{H} &= p\ddot{x} +\dot{p}\dot{x} -\lr{\pderiv{L}{t}+\pderiv{L}{x}\dot{x} + p\ddot{x}},\\
\label{5.16}
	\dot{H}  &= p\ddot{x} +\dot{p}\dot{x} -\pderiv{L}{t}-\pderiv{L}{x}\dot{x} - p\ddot{x},\\
\label{5.17}
	\dot{H} + \pderiv{L}{t} &= p\ddot{x} +\dot{p}\dot{x} -\pderiv{L}{x}\dot{x} - p\ddot{x}.
\end{align}
Multiply \eqref{5.17} by $-\tau$ and cancel like terms,
\begin{align}
\label{5.18}
	-\dot{H}\tau - \pderiv{L}{t}\tau &= \cancelto{1}{-p\ddot{x}\tau} -\dot{p}\dot{x}\tau + \pderiv{L}{x}\dot{x}\tau \cancelto{1}{+ p\ddot{x}\tau}\\
\label{5.19}
	-\dot{H}\tau - \pderiv{L}{t}\tau &=  -\dot{p}\dot{x}\tau + \pderiv{L}{x}\dot{x}\tau\\
\label{5.20}
	 - \pderiv{L}{t}\tau -\dot{H}\tau&= - \lr{\dot{p} - \pderiv{L}{x}}\dot{x}\tau
\end{align}
Substituting \eqref{5.20} into \eqref{5.10} gives,
\begin{align}
\label{5.21}
	\deriv{}{t}\lrs{p\xi-H\tau}&=  \xi\lr{\dot{p} -\pderiv{L}{x}} - \lr{\dot{p} - \pderiv{L}{x}}\dot{x}\tau.
\end{align}
Finally,
\begin{align}
\label{5.22}
	\boxed{\deriv{}{t}\lrs{p\xi-H\tau} =  \lr{\xi- \dot{x}\tau}\lr{\dot{p} -\pderiv{L}{x}},}
\end{align}
as required.

